Channel_Type_Example.thy
@@ -8,15 +8,27 @@ chantype ch_single =
 chantype ch_two =
   chbool :: bool
   chint :: int
+                      
+chantype ct =
+  a1 :: int
+  a2 :: int
+  a3 :: int
+  a4 :: int
+  a5 :: int
+  a6 :: int
+  a7 :: int
+  a8 :: int
 
 chantype ch_buffer =
   inp :: unit
   outp :: nat
-  mod :: bool
+  modif :: bool
 
 thm ch_buffer.inp_wb_prism
 
 thm ch_buffer.codeps
+
+thm ch_buffer.prism_chanreps
 
 chantype ch_buffer2 =
   inp2 :: unit
