Channel_Type_Tests.thy
@@ -1,0 +1,15 @@
+theory Channel_Type_Tests
+  imports Channel_Type
+begin
+
+(* Create a very large channel type (50 channels) to test proof and instantiation *)
+
+ML \<open> val chans = map (fn n => ("a" ^ Int.toString n, "int")) (0 upto 49); \<close>
+
+setup \<open> Channel_Type.compile_chantype ("ch_big", chans) \<close>
+
+print_theorems
+
+thm ch_big.prism_chanreps
+
+end
